direct1

theories/SLFDirect.v
@@ -85,52 +85,1006 @@ End Assumptions.
 (* ******************************************************* *)
 (** ** Syntax *)
 
+Definition loc : Type := nat.
+
+Inductive val : Type :=
+  | val_unit : val
+  | val_bool : bool -> val
+  | val_int : int -> val
+  | val_loc : loc -> val
+  | val_fun : var -> trm -> val
+  | val_fix : var -> var -> trm -> val
+  | val_ref : val
+  | val_get : val
+  | val_set : val
+  | val_add : val
+
+with trm : Type :=
+  | trm_val : val -> trm
+  | trm_var : var -> trm
+  | trm_fun : var -> trm -> trm
+  | trm_fix : var -> var -> trm -> trm
+  | trm_app : trm -> trm -> trm
+  | trm_seq : trm -> trm -> trm
+  | trm_let : var -> trm -> trm -> trm
+  | trm_if : trm -> trm -> trm -> trm.
+
+
+(* ******************************************************* *)
+(** ** Implicit Types *)
+
+Implicit Types x f : var.
+Implicit Types b : bool.
+Implicit Types l : loc.
+Implicit Types n : int.
+Implicit Types v w r : val.
+Implicit Types t : trm.
+Implicit Types s : state.
+
+
 (* ******************************************************* *)
 (** ** Substitution *)
 
-(* ******************************************************* *)
-(** ** Semantics *)
+Fixpoint subst (y:var) (w:val) (t:trm) : trm :=
+  let aux t := subst y w t in
+  let if_y_eq x t1 t2 := if var_eq x y then t1 else t2 in
+  match t with
+  | trm_val v => trm_val v
+  | trm_var x => if_y_eq x (trm_val w) t
+  | trm_fun x t1 => trm_fun x (if_y_eq x t1 (aux t1))
+  | trm_fix f x t1 => trm_fix f x (if_y_eq f t1 (if_y_eq x t1 (aux t1)))
+  | trm_app t1 t2 => trm_app (aux t1) (aux t2)
+  | trm_seq t1 t2 => trm_seq  (aux t1) (aux t2)
+  | trm_let x t1 t2 => trm_let x (aux t1) (if_y_eq x t2 (aux t2))
+  | trm_if t0 t1 t2 => trm_if (aux t0) (aux t1) (aux t2)
+  end.
+
 
 (* ******************************************************* *)
 (** ** Coercions *)
 
+Coercion trm_val : val >-> trm.
+Coercion trm_app : trm >-> Funclass.
+
+Implicit Types h : heap.
+Implicit Types H : hprop.
+Implicit Types Q : val->hprop.
+
+
 (* ******************************************************* *)
-(** ** Notations *)
+(** ** Semantics *)
+
+Inductive eval : state -> trm -> state -> val -> Prop :=
+  | eval_val : forall s v,
+      eval s (trm_val v) s v
+  | eval_fun : forall s x t1,
+      eval s (trm_fun x t1) s (val_fun x t1)
+  | eval_fix : forall s f x t1,
+      eval s (trm_fix f x t1) s (val_fix f x t1)
+  | eval_app_fun : forall s1 s2 v1 v2 x t1 v,
+      v1 = val_fun x t1 ->
+      eval s1 (subst x v2 t1) s2 v ->
+      eval s1 (trm_app v1 v2) s2 v
+  | eval_app_fix : forall s1 s2 v1 v2 f x t1 v,
+      v1 = val_fix f x t1 ->
+      eval s1 (subst x v2 (subst f v1 t1)) s2 v ->
+      eval s1 (trm_app v1 v2) s2 v
+  | eval_seq : forall s1 s2 s3 t1 t2 v1 v,
+      eval s1 t1 s2 v1 ->
+      eval s2 t2 s3 v ->
+      eval s1 (trm_seq t1 t2) s3 v
+  | eval_let : forall s1 s2 s3 x t1 t2 v1 r, 
+      eval s1 t1 s2 v1 ->
+      eval s2 (subst x v1 t2) s3 r ->
+      eval s1 (trm_let x t1 t2) s3 r
+  | eval_if_case : forall s1 s2 b v t1 t2,
+      eval s1 (if b then t1 else t2) s2 v ->
+      eval s1 (trm_if (val_bool b) t1 t2) s2 v
+  | eval_add : forall s n1 n2,
+      eval s (val_add (val_int n1) (val_int n2)) s (val_int (n1 + n2))
+  | eval_ref : forall s v l,
+      ~ Fmap.indom s l ->
+      eval s (val_ref v) (Fmap.update s l v) (val_loc l)
+  | eval_get : forall s l,
+      Fmap.indom s l ->
+      eval s (val_get (val_loc l)) s (Fmap.read s l)
+  | eval_set : forall s l v,
+      Fmap.indom s l ->
+      eval s (val_set (val_loc l) v) (Fmap.update s l v) val_unit.
 
 
 (* ####################################################### *)
 (** * Heap predicates *)
 
-(* ******************************************************* *)
-(** ** Definitions *)
+(** For technical reasons, to enable sharing the code implementing 
+    the tactic [hsimpl], we need the definitions that follow to be
+    wrapped in a module. *)
+
+Module HsimplArgs. 
+
 
 (* ******************************************************* *)
-(** ** Basic properties *)
+(** ** Hprop and entailement *)
+
+(** Type of heap predicates *)
+
+Definition hprop := heap -> Prop.
+
+(** Entailment for heap predicates *)
+
+Definition himpl (H1 H2:hprop) : Prop :=
+  forall (h:heap), H1 h -> H2 h.
+
+Notation "H1 ==> H2" := (himpl H1 H2) (at level 55).
+
+Open Scope heap_scope.
+
+(** Entailment between postconditions *)
+
+Definition qimpl A (Q1 Q2:A->hprop) : Prop :=
+  forall (v:A), Q1 v ==> Q2 v.
+
+Notation "Q1 ===> Q2" := (qimpl Q1 Q2) (at level 55).
+
+
+(* ******************************************************* *)
+(** ** Definition of heap predicates *)
+
+(** Core heap predicates *)
+
+Definition hempty : hprop :=
+  fun h => (h = Fmap.empty).
+
+Definition hsingle (l:loc) (v:val) : hprop :=
+  fun h => (h = Fmap.single l v).
+
+Definition hstar (H1 H2 : hprop) : hprop :=
+  fun h => exists h1 h2, H1 h1
+                              /\ H2 h2
+                              /\ Fmap.disjoint h1 h2
+                              /\ h = Fmap.union h1 h2.
+
+Definition hexists A (J:A->hprop) : hprop :=
+  fun h => exists x, J x h.
+
+Definition hforall (A : Type) (J : A -> hprop) : hprop :=
+  fun h => forall x, J x h.
+
+Notation "\[]" := (hempty)
+  (at level 0).
+
+Notation "l '~~~>' v" := (hsingle l v) (at level 32).
+
+Notation "H1 '\*' H2" := (hstar H1 H2)
+  (at level 41, right associativity).
+
+Notation "'\exists' x1 .. xn , H" :=
+  (hexists (fun x1 => .. (hexists (fun xn => H)) ..))
+  (at level 39, x1 binder, H at level 50, right associativity,
+   format "'[' '\exists' '/ '  x1  ..  xn , '/ '  H ']'").
+
+Notation "'\forall' x1 .. xn , H" :=
+  (hforall (fun x1 => .. (hforall (fun xn => H)) ..))
+  (at level 39, x1 binder, H at level 50, right associativity,
+   format "'[' '\forall' '/ '  x1  ..  xn , '/ '  H ']'").
+
+(** Derived heap predicates.
+
+    The following operators are defined in terms of the ones
+    above, rather than as functions over heaps, to reduce the
+    proof effort. (See the summary in [SLFWand.v] for details.) *)
+
+Definition hpure (P:Prop) : hprop :=
+  \exists (p:P), \[].
+
+Definition htop : hprop :=
+  \exists (H:hprop), H.
+
+Definition hwand (H1 H2 : hprop) : hprop :=
+  \exists H0, H0 \* \[ (H0 \* H1) ==> H2].
+
+Definition qwand A (Q1 Q2:A->hprop) :=
+  \forall x, hwand (Q1 x) (Q2 x).
+
+Notation "\[ P ]" := (hpure P)
+  (at level 0, format "\[ P ]").
+
+Notation "\Top" := (htop).
+
+Notation "Q \*+ H" := (fun x => hstar (Q x) H)
+  (at level 40).
+
+Notation "H1 \-* H2" := (hwand H1 H2)
+  (at level 43, right associativity).
+
+Notation "Q1 \--* Q2" := (qwand Q1 Q2)
+  (at level 43).
+
+
+(* ******************************************************* *)
+(** ** Basic properties of Separation Logic operators *)
+
+(* ---------------------------------------------------------------------- *)
+(* ** Properties of [himpl] *)
+
+Lemma himpl_refl : forall H,
+  H ==> H.
+Proof using. introv M. auto. Qed.
+
+Lemma himpl_trans : forall H2 H1 H3,
+  (H1 ==> H2) ->
+  (H2 ==> H3) ->
+  (H1 ==> H3).
+Proof using. introv M1 M2. intros h H1h. eauto. Qed.
+
+Lemma himpl_antisym : forall H1 H2,
+  (H1 ==> H2) ->
+  (H2 ==> H1) ->
+  (H1 = H2).
+Proof using. introv M1 M2. applys pred_ext_1. intros h. iff*. Qed.
+
+Lemma himpl_forall_trans : forall H1 H2,
+  (forall H, H ==> H1 -> H ==> H2) ->
+  H1 ==> H2.
+Proof using. introv M. applys~ M. Qed.
+
+
+(* ---------------------------------------------------------------------- *)
+(* ** Properties of [hstar] *)
+
+Lemma hstar_hempty_r : forall H,
+  H \* \[] = H.
+Proof using.
+  applys neutral_r_of_comm_neutral_l.
+  applys~ hstar_comm.
+  applys~ hstar_hempty_l.
+Qed.
+
+Lemma himpl_frame_r : forall H1 H2 H2',
+  H2 ==> H2' ->
+  (H1 \* H2) ==> (H1 \* H2').
+Proof using.
+  introv M. do 2 rewrite (@hstar_comm H1). applys~ himpl_frame_l.
+Qed.
+
+Lemma himpl_frame_lr : forall H1 H1' H2 H2',
+  H1 ==> H1' ->
+  H2 ==> H2' ->
+  (H1 \* H2) ==> (H1' \* H2').
+Proof using.
+  introv M1 M2. applys himpl_trans. applys~ himpl_frame_l M1. applys~ himpl_frame_r.
+Qed.
+
+Lemma himpl_hstar_trans_l : forall H1 H2 H3 H4,
+  H1 ==> H2 ->
+  H2 \* H3 ==> H4 ->
+  H1 \* H3 ==> H4.
+Proof using.
+  introv M1 M2. applys himpl_trans M2. applys himpl_frame_l M1. 
+Qed.
+
+Lemma himpl_hstar_trans_r : forall H1 H2 H3 H4,
+  H1 ==> H2 ->
+  H3 \* H2 ==> H4 ->
+  H3 \* H1 ==> H4.
+Proof using.
+  introv M1 M2. applys himpl_trans M2. applys himpl_frame_r M1. 
+Qed.
+
+
+(* ---------------------------------------------------------------------- *)
+(** Properties of [hpure] *)
+
+Lemma hstar_hpure : forall P H h, 
+  (\[P] \* H) h = (P /\ H h).
+Proof using.
+  intros. extens. unfold hpure.
+  rewrite hstar_hexists.
+  rewrite* hstar_hempty_l.
+  iff (p&M) (p&M). { split~. } { exists~ p. }
+Qed.
+
+Lemma hstar_hpure_iff : forall P H h,
+  (\[P] \* H) h <-> (P /\ H h).
+Proof using. intros. rewrite* hstar_hpure. Qed.
+
+Lemma himpl_hstar_hpure_r : forall P H H',
+  P ->
+  (H ==> H') ->
+  H ==> (\[P] \* H').
+Proof using.
+  introv HP W. intros h K. rewrite* hstar_hpure.
+Qed.
+
+Lemma hpure_inv_hempty : forall P h,
+  \[P] h ->
+  P /\ \[] h.
+Proof using.
+  introv M. rewrite <- hstar_hpure.
+  rewrite~ hstar_hempty_r.
+Qed.
+
+Lemma hpure_intro_hempty : forall P h,
+  \[] h ->
+  P ->
+  \[P] h.
+Proof using.
+  introv M N. rewrite <- (hstar_hempty_l \[P]).
+  rewrite hstar_comm. rewrite~ hstar_hpure.
+Qed.
+
+Lemma himpl_hempty_hpure : forall P,
+  P ->
+  \[] ==> \[P].
+Proof using. introv HP. intros h Hh. applys* hpure_intro_hempty. Qed.
+
+Lemma himpl_hstar_hpure_l : forall P H H',
+  (P -> H ==> H') ->
+  (\[P] \* H) ==> H'.
+Proof using.
+  introv W Hh. rewrite hstar_hpure in Hh. applys* W.
+Qed.
+
+Lemma hempty_eq_hpure_true :
+  \[] = \[True].
+Proof using.
+  applys pred_ext_1. intros h. iff M.
+  { applys* hpure_intro_hempty. }
+  { forwards*: hpure_inv_hempty M. }
+Qed.
+
+Lemma hfalse_hstar_any : forall H,
+  \[False] \* H = \[False].
+Proof using.
+  intros. applys pred_ext_1. intros h. rewrite hstar_hpure. iff M.
+  { false*. } { lets: hpure_inv_hempty M. false*. }
+Qed.
+
+
+(* ---------------------------------------------------------------------- *)
+(** Properties of hexists *)
+
+Lemma hexists_intro : forall A (x:A) (J:A->hprop) h,
+  J x h ->
+  (hexists J) h.
+Proof using. intros. exists~ x. Qed.
+
+Lemma hexists_inv : forall A (J:A->hprop) h,
+  (hexists J) h ->
+  exists x, J x h.
+Proof using. intros. destruct H as [x H]. exists~ x. Qed.
+
+Lemma himpl_hexists_l : forall A H (J:A->hprop),
+  (forall x, J x ==> H) ->
+  (hexists J) ==> H.
+Proof using. introv W. intros h (x&Hh). applys* W. Qed.
+
+Lemma himpl_hexists_r : forall A (x:A) H J,
+  (H ==> J x) ->
+  H ==> (hexists J).
+Proof using. introv W. intros h. exists x. apply~ W. Qed.
+
+(* not needed *)
+Lemma himpl_hexists : forall A (J1 J2:A->hprop),
+  J1 ===> J2 ->
+  hexists J1 ==> hexists J2.
+Proof using.
+  introv W. applys himpl_hexists_l. intros x. applys himpl_hexists_r W.
+Qed.
+
+
+(* ---------------------------------------------------------------------- *)
+(** Properties of hforall *)
+
+Lemma himpl_hforall_r : forall A (J:A->hprop) H,
+  (forall x, H ==> J x) ->
+  H ==> (hforall J).
+Proof using. introv M. intros h Hh x. apply~ M. Qed.
+
+Lemma himpl_hforall_l : forall A x (J:A->hprop) H,
+  (J x ==> H) ->
+  (hforall J) ==> H.
+Proof using. introv M. intros h Hh. apply~ M. Qed.
+
+Lemma hforall_specialize : forall A (x:A) (J:A->hprop),
+  (hforall J) ==> (J x).
+Proof using. intros. applys* himpl_hforall_l x. Qed.
+
+(* not needed *)
+Lemma himpl_hforall : forall A (J1 J2:A->hprop),
+  J1 ===> J2 ->
+  hforall J1 ==> hforall J2.
+Proof using.
+  introv W. applys himpl_hforall_r. intros x. applys himpl_hforall_l W.
+Qed.
+
+
+(* ---------------------------------------------------------------------- *)
+(** Properties of hwand (others are found further in the file) *)
+
+Lemma hwand_equiv : forall H0 H1 H2,
+  (H0 ==> H1 \-* H2) <-> (H0 \* H1 ==> H2).
+Proof using.
+  unfold hwand. iff M.
+  { applys himpl_trans. applys himpl_frame_l M.
+    (* applys himpl_hstar_trans_l (rm M). *)
+    rewrite hstar_hexists. applys himpl_hexists_l. intros H.
+    rewrite (hstar_comm H). rewrite hstar_assoc.
+    applys~ himpl_hstar_hpure_l. }
+  { applys himpl_hexists_r H0. 
+    rewrite hstar_comm. rewrite <- (hstar_hempty_l H0) at 1.
+    applys himpl_frame_l. applys himpl_hempty_hpure M. }
+Qed.
+
+Lemma himpl_hwand_r : forall H1 H2 H3,
+  H1 \* H2 ==> H3 ->
+  H1 ==> (H2 \-* H3).
+Proof using. introv M. rewrite~ hwand_equiv. Qed.
+
+Lemma himpl_hwand_r_inv : forall H1 H2 H3,
+  H1 ==> (H2 \-* H3) ->
+  H1 \* H2 ==> H3.
+Proof using. introv M. rewrite~ <- hwand_equiv. Qed.
+
+Lemma hwand_cancel : forall H1 H2,
+  H1 \* (H1 \-* H2) ==> H2.
+Proof using. intros. rewrite hstar_comm. rewrite~ <- hwand_equiv. Qed.
+
+Arguments hwand_cancel : clear implicits.
+
+Lemma himpl_hempty_hwand_same : forall H,
+  \[] ==> (H \-* H).
+Proof using. intros. rewrite hwand_equiv. rewrite~ hstar_hempty_l. Qed.
+
+Lemma hwand_hempty_l : forall H,
+  (\[] \-* H) = H.
+Proof using.
+  intros. applys himpl_antisym.
+  { rewrite <- (hstar_hempty_l (\[] \-* H)). applys hwand_cancel. }
+  { rewrite hwand_equiv. rewrite~ hstar_hempty_r. }
+Qed.
+
+Lemma hwand_hpure_l_intro : forall (P:Prop) H,
+  P ->
+  \[P] \-* H ==> H.
+Proof using. 
+  introv HP. rewrite <- (hstar_hempty_l (\[P] \-* H)).
+  forwards~ K: himpl_hempty_hpure P.
+  applys* himpl_hstar_trans_l K. applys hwand_cancel.
+Qed.
+
+Arguments hwand_hpure_l_intro : clear implicits.
+
+Lemma hwand_curry : forall H1 H2 H3,
+  (H1 \* H2) \-* H3 ==> H1 \-* (H2 \-* H3).
+Proof using.
+  intros. do 2 rewrite hwand_equiv.
+  rewrite hstar_assoc. rewrite hstar_comm. applys hwand_cancel.
+Qed.
+
+Lemma hwand_uncurry : forall H1 H2 H3,
+  H1 \-* (H2 \-* H3) ==> (H1 \* H2) \-* H3.
+Proof using.
+  intros. rewrite hwand_equiv. rewrite <- (hstar_comm (H1 \* H2)). 
+  rewrite (@hstar_comm H1). rewrite hstar_assoc.
+  applys himpl_trans. applys himpl_frame_r. applys hwand_cancel.
+  applys hwand_cancel.
+Qed.
+
+Lemma hwand_curry_eq : forall H1 H2 H3,
+  (H1 \* H2) \-* H3 = H1 \-* (H2 \-* H3).
+Proof using.
+  intros. applys himpl_antisym.
+  { applys hwand_curry. }
+  { applys hwand_uncurry. }
+Qed.
+
+
+(* ---------------------------------------------------------------------- *)
+(** Properties of qwand *)
+
+Lemma qwand_equiv : forall H A (Q1 Q2:A->hprop),
+  H ==> (Q1 \--* Q2) <-> (Q1 \*+ H) ===> Q2.
+Proof using.
+  unfold qwand. iff M.
+  { intros x. rewrite hstar_comm. applys himpl_trans.
+    applys himpl_frame_l M. applys himpl_trans. applys hstar_hforall.
+    applys himpl_hforall_l x. rewrite <- hwand_equiv. applys himpl_refl. }
+  { applys himpl_hforall_r. intros x.
+    rewrite hwand_equiv. rewrite* hstar_comm. }
+Qed.
+
+Lemma himpl_qwand_r : forall A (Q1 Q2:A->hprop) H,
+  Q1 \*+ H ===> Q2 ->
+  H ==> (Q1 \--* Q2).
+Proof using. introv M. rewrite~ qwand_equiv. Qed.
+
+Arguments himpl_qwand_r [A].
+
+Lemma qwand_specialize : forall A (x:A) (Q1 Q2:A->hprop),
+  (Q1 \--* Q2) ==> (Q1 x \-* Q2 x).
+Proof using.
+  intros. applys himpl_forall_trans. intros H M.
+  rewrite qwand_equiv in M. specializes M x.
+  rewrite hwand_equiv. rewrite~ hstar_comm.
+Qed.
+
+Arguments qwand_specialize [ A ].
+
+
+(* ---------------------------------------------------------------------- *)
+(** Properties of htop *)
+
+Lemma htop_intro : forall h,
+  \Top h.
+Proof using. intros. exists~ (=h). Qed.
+
+Lemma himpl_htop_r : forall H,
+  H ==> \Top.
+Proof using. intros. intros h Hh. applys* htop_intro. Qed.
+
+Lemma htop_eq :
+  \Top = (\exists H, H).
+Proof using. auto. Qed.
+
+Lemma hstar_htop_htop :
+  \Top \* \Top = \Top.
+Proof using.
+  applys himpl_antisym.
+  { applys himpl_htop_r. }
+  { applys himpl_forall_trans. intros H M. applys himpl_trans M.
+    rewrite <- (hstar_hempty_r \Top) at 1. applys himpl_frame_r.
+    applys himpl_htop_r. }
+Qed.
+
 
 (* ******************************************************* *)
 (** ** Hsimpl tactic *)
+
+(** The definitions and properties above enable us to instantiate
+    the [hsimpl] tactic, which implements powerful simplifications
+    for Separation Logic entailments. 
+    
+    For technical reasons, we need to provide a definition for [hgc],
+    a restriction of [htop] to affine heap predicates. For our purpose,
+    it suffices to define [hgc] as an alias for [htop]. *)
+
+(* ---------------------------------------------------------------------- *)
+(** Definition and properties of hgc *)
+
+Definition hgc := htop.
+
+Definition haffine := fun H => True.
+
+Lemma haffine_hempty :
+  haffine \[].
+Proof using. hnfs*. Qed.
+
+Lemma himpl_hgc_r : forall H,
+  haffine H ->
+  H ==> \GC.
+Proof using. introv M. applys himpl_htop_r. Qed.
+
+Lemma hstar_hgc_hgc :
+  \GC \* \GC = \GC.
+Proof using. applys hstar_htop_htop. Qed.
+
+
+(* ---------------------------------------------------------------------- *)
+(** Functor instantiation to obtain [hsimpl] *)
+
+End HsimplArgs. 
+
+(** We are now ready to instantiate the functor. *)
+
+Module Export HS := HsimplSetup(HsimplArgs).
+
+(** At this point, the tactic [hsimpl] is available.
+    See the file [SLFHimpl.v] for demos of its usage. *)  
+
+(** And we open the module [HsimplArgs], essentially pretending
+    that it was never created. *)
+
+Export HsimplArgs.
 
 
 (* ####################################################### *)
 (** * Reasoning rules *)
 
+
+(* ******************************************************* *)
+(** ** Evaluation rules for primitives in Separation style *)
+
+(** It is not needed to follow through these proofs. *)
+
+Lemma eval_get_sep : forall s s2 l v, 
+  s = (Fmap.single l v) \u s2 ->
+  eval s (val_get (val_loc l)) s v.
+Proof using.
+  introv ->. forwards Dv: Fmap.indom_single l v.
+  applys_eq eval_get 1.
+  { applys~ Fmap.indom_union_l. }
+  { rewrite~ Fmap.read_union_l. rewrite~ Fmap.read_single. }
+Qed.
+
+Lemma eval_set_sep : forall s1 s2 h2 l v1 v2,
+  s1 = Fmap.union (Fmap.single l v1) h2 ->
+  s2 = Fmap.union (Fmap.single l v2) h2 ->
+  Fmap.disjoint (Fmap.single l v1) h2 ->
+  eval s1 (val_set (val_loc l) v2) s2 val_unit.
+Proof using.
+  introv -> -> D. forwards Dv: Fmap.indom_single l v1.
+  applys_eq eval_set 2.
+  { applys~ Fmap.indom_union_l. }
+  { rewrite~ Fmap.update_union_l. fequals.
+    rewrite~ Fmap.update_single. }
+Qed.
+
+Lemma eval_ref_sep : forall s1 s2 v l,
+  s2 = Fmap.single l v ->
+  Fmap.disjoint s2 s1 ->
+  eval s1 (val_ref v) (Fmap.union s2 s1) (val_loc l).
+Proof using.
+  (** It is not needed to follow through this proof. *)
+  introv -> D. forwards Dv: Fmap.indom_single l v.
+  rewrite <- Fmap.update_eq_union_single. applys~ eval_ref.
+  { intros N. applys~ Fmap.disjoint_inv_not_indom_both D N. }
+Qed.
+
+
 (* ******************************************************* *)
 (** ** Hoare reasoning rules *)
 
-(* ******************************************************* *)
-(** ** Definition of WP and SL triple *)
+(** * Definition of Hoare triples *)
+
+Definition hoare (t:trm) (H:hprop) (Q:val->hprop) :=
+  forall h, H h -> exists h' v, eval h t h' v /\ Q v h'.
+
+(** The tactic [himpl_fold] applies to a goal of the form [H1 h].
+    It searches the context for an assumption of the from [H2 h],
+    then replaces the goal with [H1 ==> H2].
+    It also deletes the assumption [H2 h]. *)
+
+Ltac himpl_fold_core tt :=
+  match goal with N: ?H ?h |- _ ?h =>
+    applys himpl_inv N; clear N end.
+
+Tactic Notation "himpl_fold" := himpl_fold_core tt.
+Tactic Notation "himpl_fold" "~" := himpl_fold; auto_tilde.
+Tactic Notation "himpl_fold" "*" := himpl_fold; auto_star.
+
+Lemma hoare_conseq : forall t H' Q' H Q,
+  hoare t H' Q' ->
+  H ==> H' ->
+  Q' ===> Q ->
+  hoare t H Q.
+Proof using.
+  introv M MH MQ HF. forwards (h'&v&R&K): M h.
+  { himpl_fold~. }
+  exists h' v. splits~. { himpl_fold. auto. }
+Qed.
+
+Lemma hoare_val : forall v H Q,
+  H ==> Q v ->
+  hoare (trm_val v) H Q.
+Proof using.
+  introv M. intros h Hh. exists h v. splits.
+  { applys eval_val. }
+  { himpl_fold~. }
+Qed.
+
+Lemma hoare_fun : forall x t1 H Q,
+  H ==> Q (val_fun x t1) ->
+  hoare (trm_fun x t1) H Q.
+Proof using.
+  introv N M. intros h Hh. exists___. splits.
+  { applys~ eval_fun. }
+  { himpl_fold~. }
+Qed.
+
+Lemma hoare_fix : forall f x t1 H Q,
+  H ==> Q (val_fix f x t1) ->
+  hoare (trm_fix f x t1) H Q.
+Proof using.
+  introv N M. intros h Hh. exists___. splits.
+  { applys~ eval_fix. }
+  { himpl_fold~. }
+Qed.
+
+Lemma hoare_seq : forall t1 t2 H Q H1,
+  hoare t1 H (fun r => H1) ->
+  hoare t2 H1 Q ->
+  hoare (trm_seq t1 t2) H Q.
+Proof using.
+  introv M1 M2 Hh.
+  forwards* (h1'&v1&R1&K1): (rm M1).
+  forwards* (h2'&v2&R2&K2): (rm M2).
+  exists h2' v2. splits~. { applys~ eval_seq R2. }
+Qed.
+
+Lemma hoare_let : forall z t1 t2 H Q Q1,
+  hoare t1 H Q1 ->
+  (forall v, hoare (subst1 z v t2) (Q1 v) Q) ->
+  hoare (trm_let z t1 t2) H Q.
+Proof using.
+  introv M1 M2 Hh.
+  forwards* (h1'&v1&R1&K1): (rm M1).
+  forwards* (h2'&v2&R2&K2): (rm M2).
+  exists h2' v2. splits~. { applys~ eval_let R2. }
+Qed.
+
+Lemma hoare_if_case : forall (b:bool) t1 t2 H Q,
+  hoare (if b then t1 else t2) H Q ->
+  hoare (trm_if b t1 t2) H Q.
+Proof using.
+  introv M1. intros h Hh. forwards* (h1'&v1&R1&K1): (rm M1).
+  exists h1' v1. splits~. { applys* eval_if. }
+Qed.
+
+Lemma hoare_add : forall H n1 n2,
+  hoare (val_add n1 n2)
+    H
+    (fun r => \[r = val_int (n1 + n2)] \* H).
+Proof using.
+  intros. intros s K0. exists s (val_int (n1 + n2)). split.
+  { applys eval_add. }
+  { rewrite hstar_hpure_iff. split.
+    { auto. }
+    { applys K0. } }
+Qed.
+
+Lemma hoare_ref : forall H v,
+  hoare (val_ref v)
+    H
+    (fun r => (\exists l, \[r = val_loc l] \* l ~~~> v) \* H).
+Proof using.
+  (* 1. We unfold the definition of [hoare]. *)
+  intros. intros s1 K0.
+  (* 2. We claim the disjointness relation 
+       [Fmap.disjoint (Fmap.single l v) s1]. *)
+  forwards~ (l&D): (single_fresh s1 v).
+  (* 3. We provide the witnesses for the reduction,
+        as dictated by [red_ref_sep]. *)
+  exists ((Fmap.single l v) \u s1) (val_loc l). split.
+  { (* 4. We exploit [red_ref_sep], which has exactly the desired shape! *)
+    applys eval_ref_sep D. auto. }
+  { (* 5. We establish the postcondition 
+       [(\exists l, \[r = val_loc l] \* l ~~~> v) \* H]
+       by providing [p] and the relevant pieces of heap. *)
+    applys hstar_intro.
+    { exists l. rewrite hstar_hpure.
+      split. { auto. } { applys hsingle_intro. } }
+    { applys K0. }
+    { applys D. } }
+Qed.
+
+Lemma hoare_get : forall H v l,
+  hoare (val_get l)
+    ((l ~~~> v) \* H)
+    (fun r => \[r = v] \* (l ~~~> v) \* H).
+Proof using.
+  (* 1. We unfold the definition of [hoare]. *)
+  intros. intros s K0. 
+  (* 2. We provide the witnesses for the reduction,
+        as dictated by [red_get_sep]. *)
+  exists s v. split.
+  { (* 3. To justify the reduction using [red_get_sep], we need to
+          argue that the state [s] decomposes as a singleton heap
+          [Fmap.single l v] and the rest of the state [s2]. This is
+          obtained by eliminating the star in hypothesis [K0]. *)
+    destruct K0 as (s1&s2&P1&P2&D&U).
+    (*    and subsequently inverting [(l ~~~> v) h1]. *)
+    lets E1: hsingle_inv P1. subst s1.
+    (* 4. At this point, the goal matches exactly [red_get_sep]. *)
+    applys eval_get_sep U. }
+  { (* 5. To establish the postcondition, we reuse justify the
+          pure fact \[v = v], and check that the state, which
+          has not changed, satisfy the same heap predicate as
+          in the precondition. *)
+    rewrite hstar_hpure. auto. }
+Qed.
+
+
+Lemma hoare_set : forall H w l v,
+  hoare (val_set (val_loc l) w)
+    ((l ~~~> v) \* H)
+    (fun r => \[r = val_unit] \* (l ~~~> w) \* H).
+Proof using. 
+  (* 1. We unfold the definition of [hoare]. *)
+  intros. intros s1 K0.
+  (* 2. We decompose the star from the precondition. *)
+  destruct K0 as (h1&h2&P1&P2&D&U).
+  (* 3. We also decompose the singleton heap predicate from it. *)
+  lets E1: hsingle_inv P1.
+  (* 4. We provide the witnesses as guided by [red_set_sep]. *)
+  exists ((Fmap.single l w) \u h2) val_unit. split.
+  { (* 5. The evaluation subgoal matches the statement of [red_set_sep]. *)
+    subst h1. applys eval_set_sep U D. auto. }
+  { (* 6. To establish the postcondition, we first isolate the pure fact. *)
+    rewrite hstar_hpure. split.
+    { auto. }
+    { (* 7. Then establish the star. *)
+      applys hstar_intro.
+      { (* 8. We establish the heap predicate [l ~~~> w] *) 
+        applys hsingle_intro. }
+      { applys P2. }
+      { (* 9. Finally, we justify disjointness using the lemma 
+              [Fmap.disjoint_single_set] introduced earlier. *)
+        subst h1. applys Fmap.disjoint_single_set D. } } }
+Qed.
+
 
 (* ******************************************************* *)
-(** ** WP-style structural properties *)
+(** ** Definition of [wp] and reasoning rules *)
+
+
+(* ---------------------------------------------------------------------- *)
+(** Definition of [wp] w.r.t. [hoare]  *)
+
+Definition wp (t:trm) := fun (Q:val->hprop) =>
+  \exists H, H \* \[forall H', hoare t (H \* H') (Q \*+ H' \*+ \Top)].
+
+
+(* ---------------------------------------------------------------------- *)
+(** Structural rule for [wp]. *)
+
+Lemma wp_ramified : forall t Q1 Q2,
+  (wp t Q1) \* (Q1 \--* Q2 \*+ \Top) ==> (wp t Q2).
+Proof using.
+  intros. do 2 rewrite wp_def. hpull ;=> H M.
+  hsimpl (H \* (Q1 \--* Q2 \*+ \Top)). intros H'.
+  applys hoare_conseq M; hsimpl.
+Qed.
+
+(* ---------------------------------------------------------------------- *)
+(** Reasoning rules for terms. *)
+
+Lemma wp_val : forall v Q,
+  Q v ==> wp (trm_val v) Q.
+Proof using. intros. rewrite wp_def. hsimpl; intros H'. applys hoare_val. hsimpl. Qed.
+
+Lemma wp_fun : forall x t Q,
+  Q (val_fun x t) ==> wp (trm_fun x t) Q.
+Proof using. intros. rewrite wp_def. hsimpl; intros H'. applys hoare_fun. hsimpl. Qed.
+
+Lemma wp_fix : forall f x t Q,
+  Q (val_fix f x t) ==> wp (trm_fix f x t) Q.
+Proof using. intros. rewrite wp_def. hsimpl; intros H'. applys hoare_fix. hsimpl. Qed.
+
+Lemma wp_if_case : forall b t1 t2 Q,
+  wp (if b then t1 else t2) Q ==> wp (trm_if b t1 t2) Q.
+Proof using.
+  intros. repeat rewrite wp_def. hsimpl; intros H M H'.
+  applys hoare_if_case. applys M.
+Qed.
+
+Lemma wp_if : forall b t1 t2 Q,
+  (if b then wp t1 Q else wp t2 Q) ==> wp (trm_if b t1 t2) Q.
+Proof using. intros. applys himpl_trans wp_if_case. case_if~. Qed.
+
+Lemma wp_seq : forall t1 t2 Q,
+  wp t1 (fun r => wp t2 Q) ==> wp (trm_seq t1 t2) Q.
+Proof using.
+  intros. rewrite wp_def. hsimpl. intros H' M1.
+  rewrite wp_def. hsimpl. intros H''.
+  applys hoare_seq. applys (rm M1). rewrite wp_def.
+  repeat rewrite hstar_hexists. applys hoare_hexists; intros H'''.
+  rewrite (hstar_comm H'''); repeat rewrite hstar_assoc.
+  applys hoare_hpure; intros M2. applys hoare_conseq M2; hsimpl.
+Qed.
+
+Lemma wp_let : forall x t1 t2 Q,
+  wp t1 (fun v => wp (subst x v t2) Q) ==> wp (trm_let x t1 t2) Q.
+Proof using.
+  intros. rewrite wp_def. hsimpl. intros H' M1.
+  rewrite wp_def. hsimpl. intros H''.
+  applys hoare_let. applys (rm M1). intros v. simpl.
+  rewrite wp_def.
+  repeat rewrite hstar_hexists. applys hoare_hexists; intros H'''.
+  rewrite (hstar_comm H'''); repeat rewrite hstar_assoc.
+  applys hoare_hpure; intros M2. applys hoare_conseq M2; hsimpl.
+Qed.
+
+
+(* ---------------------------------------------------------------------- *)
+(** Rules for primitives. *)
+
+Lemma hoare_set : forall H w l v,
+  hoare (val_set (val_loc l) w)
+    ((l ~~~> v) \* H)
+    (fun r => \[r = val_unit] \* (l ~~~> w) \* H).
+Proof using. 
+  (* 1. We unfold the definition of [hoare]. *)
+  intros. intros s1 K0.
+  (* 2. We decompose the star from the precondition. *)
+  destruct K0 as (h1&h2&P1&P2&D&U).
+  (* 3. We also decompose the singleton heap predicate from it. *)
+  lets E1: hsingle_inv P1.
+  (* 4. We provide the witnesses as guided by [red_set_sep]. *)
+  exists ((Fmap.single l w) \u h2) val_unit. split.
+  { (* 5. The evaluation subgoal matches the statement of [red_set_sep]. *)
+    subst h1. applys eval_set_sep U D. auto. }
+  { (* 6. To establish the postcondition, we first isolate the pure fact. *)
+    rewrite hstar_hpure. split.
+    { auto. }
+    { (* 7. Then establish the star. *)
+      applys hstar_intro.
+      { (* 8. We establish the heap predicate [l ~~~> w] *) 
+        applys hsingle_intro. }
+      { applys P2. }
+      { (* 9. Finally, we justify disjointness using the lemma 
+              [Fmap.disjoint_single_set] introduced earlier. *)
+        subst h1. applys Fmap.disjoint_single_set D. } } }
+Qed.
+
+
 
 (* ******************************************************* *)
-(** ** WP-style reasoning rules for terms *)
+(** ** Definition of triple and equivalence *)
+
+Definition triple (t:trm) (H:hprop) (Q:val->hprop) : Prop :=
+  forall (H':hprop), hoare t (H \* H') (Q \*+ H' \*+ \Top).
+
+Lemma wp_equiv : forall t H Q,
+  (triple t H Q) <-> (H ==> wp t Q).
+Proof using.
+  iff M.
+  { hsimpl H. apply M. }
+  { applys triple_conseq Q M.
+    { applys triple_hexists. intros H'.
+      rewrite hstar_comm. applys triple_hpure. 
+      intros N. applys N. }
+    { applys qimpl_refl. } }
+Qed.
+
 
 (* ******************************************************* *)
 (** ** Specification for primitive functions *)
 
-(* ******************************************************* *)
-(** ** WP reasoning rules *)
+Lemma triple_add' : forall n1 n2,
+  triple (val_add n1 n2)
+    \[]
+    (fun r => \[r = val_int (n1 + n2)]).
+Proof using.
+  rewrite wp_equiv.
+  intros. applys triple_of_hoare. intros H'. esplit. split.
+  applys hoare_add. hsimpl. auto.
+(* /SOLUTION *)
+Qed.
+
+Lemma triple_ref : forall v,
+  triple (val_ref v)
+    \[]
+    (fun r => \exists l, \[r = val_loc l] \* l ~~~> v).
+Proof using.
+  intros. intros H'. applys hoare_conseq.
+  { applys hoare_ref. } 
+  { hsimpl. }
+  { hsimpl. auto. }
+Qed.
+
+Lemma triple_get : forall v l,
+  triple (val_get l)
+    (l ~~~> v)
+    (fun r => \[r = v] \* (l ~~~> v)).
+Proof using.
+  intros. intros H'. applys hoare_conseq.
+  { applys hoare_get. } 
+  { hsimpl. }
+  { hsimpl. auto. }
+Qed.
+
+Lemma triple_set : forall w l v,
+  triple (val_set (val_loc l) w)
+    (l ~~~> v)
+    (fun r => \[r = val_unit] \* l ~~~> w).
+Proof using.
+  intros. intros H'. applys hoare_conseq.
+  { applys hoare_set. } 
+  { hsimpl. }
+  { hsimpl. auto. }
+Qed.
+
 
 
 (* ####################################################### *)
@@ -147,6 +1101,13 @@ End Assumptions.
 
 (* ******************************************************* *)
 (** ** Tactics *)
+
+
+(* ####################################################### *)
+(** * Practical proofs *)
+
+(* ******************************************************* *)
+(** ** Notation for terms *)
 
 (* ******************************************************* *)
 (** ** Example proof *)
